backend/Unusedglobproof.v
@@ -343,7 +343,7 @@ Lemma filter_globdefs_map_1:
   forall id l u m1 m2,
   IS.mem id u = false ->
   m1! id = option_map remove_gfun m2!id ->
-  (fold_left add_def (filter_globdefs u l) m1)!id = 
+  (fold_left add_def (filter_globdefs u l) m1)!id =
   option_map remove_gfun (fold_left add_def l m2)!id.
 Proof.
   induction l as [ | [id1 gd1] l]; simpl; intros.
@@ -365,21 +365,21 @@ Lemma filter_globdefs_map_2:
 Proof.
   induction l as [ | [id1 gd1] l]; simpl; intros.
 - auto.
-- simpl. 
+- simpl.
   destruct (IS.mem id1 u) eqn:MEM.
   + apply IHl; auto.
-    unfold filter_globdefs. 
+    unfold filter_globdefs.
     unfold add_def at 1 2. simpl.
     rewrite ! PTree.gsspec. destruct (peq id id1). auto. auto.
   + apply IHl; auto. unfold add_def. simpl.
-     destruct (peq id id1). congruence. 
+     destruct (peq id id1). congruence.
     rewrite !PTree.gso by congruence. auto.
 Qed.
 
 Lemma filter_globdefs_map:
   forall id u defs,
   (PTree_Properties.of_list (filter_globdefs u defs))! id =
-  if IS.mem id u then (PTree_Properties.of_list defs)!id 
+  if IS.mem id u then (PTree_Properties.of_list defs)!id
                  else option_map remove_gfun (PTree_Properties.of_list defs)!id.
 Proof.
   intros. unfold PTree_Properties.of_list. fold prog_map. unfold PTree.elt. fold add_def.
@@ -409,7 +409,7 @@ Qed.
 Section ORACLE.
 Variable fn_stack_requirements : ident -> Z.
 
-Require Import LanguageInterface Inject.
+Require Import LanguageInterface Inject InjectFootprint.
 
 (** The initial memory injection inferred from global symbol tables *)
 Definition init_meminj (se tse: Genv.symtbl) : meminj :=
@@ -442,7 +442,7 @@ Hypothesis GE: inj_stbls w se tse.
 Hypothesis VALID: Genv.valid_for skel se.
 
 Lemma main_symb_pres: forall b,
-    Genv.find_symbol se (prog_main skel) = Some b -> 
+    Genv.find_symbol se (prog_main skel) = Some b ->
     exists b', Genv.find_symbol tse (prog_main tskel) = Some b'.
 Proof.
   intros. inv GE. inv inj_stbls_match.
@@ -490,8 +490,8 @@ Proof.
 Qed.
 
 Lemma remove_unused_consistent: forall id gd b,
-    (prog_defmap skel) ! id = Some gd -> 
-    Genv.find_symbol tse id = Some b -> 
+    (prog_defmap skel) ! id = Some gd ->
+    Genv.find_symbol tse id = Some b ->
     (prog_defmap tskel) ! id = Some gd.
 Proof.
   intros. simpl.
@@ -504,8 +504,8 @@ Qed.
 
 
 Lemma remove_unused_consistent_p :forall id gd b,
-    (prog_defmap p) ! id = Some gd -> 
-    Genv.find_symbol tse id = Some b -> 
+    (prog_defmap p) ! id = Some gd ->
+    Genv.find_symbol tse id = Some b ->
     (prog_defmap tp) ! id = Some gd.
 Proof.
   intros.
@@ -519,7 +519,7 @@ Proof.
   unfold option_map in TDEF.
   destruct ((prog_defmap tp) ! id) eqn:TDEF'; try discriminate.
   inv TDEF.
-  inv TRANSF. 
+  inv TRANSF.
   rewrite (match_prog_def0 id) in TDEF'.
   destruct (IS.mem id used) eqn:MEM; try discriminate.
   rewrite H in TDEF'. inv TDEF'.
@@ -528,7 +528,7 @@ Proof.
 Qed.
 
 (** Public symbols of source and target symbol tables are the same *)
-Lemma se_public_same: forall id, 
+Lemma se_public_same: forall id,
     Genv.public_symbol se id = Genv.public_symbol tse id.
 Proof.
   intros. symmetry. inv GE. inv inj_stbls_match. eauto.
@@ -590,9 +590,9 @@ Proof.
 Qed.
 
 Lemma symbols_inject_init_public: forall id b,
-    Genv.public_symbol se id = true -> 
+    Genv.public_symbol se id = true ->
     Genv.find_symbol se id = Some b ->
-    exists b', Genv.find_symbol tse id = Some b' /\ 
+    exists b', Genv.find_symbol tse id = Some b' /\
           init_meminj se tse b = Some(b', 0).
 Proof.
   cbn.
@@ -619,13 +619,10 @@ Qed.
 (** Injections that preserve used globals. *)
 
 Record meminj_preserves_globals (f: meminj) : Prop := {
-<<<<<<< HEAD
   (** Invariants for global injections *)
-=======
-  symbols_inject_0: forall id b' delta,
+  (* symbols_inject_0: forall id b' delta,
     f (Global id) = Some (b', delta) -> sup_In (Global id) (Genv.genv_sup ge) ->
-      b' = Global id /\ delta = 0;  
->>>>>>> origin/StackAware-new
+      b' = Global id /\ delta = 0;   *)
   symbols_inject_1: forall id b b' delta,
     f b = Some(b', delta) -> Genv.find_symbol ge id = Some b ->
     delta = 0 /\ Genv.find_symbol tge id = Some b';
@@ -633,7 +630,7 @@ Record meminj_preserves_globals (f: meminj) : Prop := {
     Genv.find_symbol tge id = Some b' ->
     exists b, Genv.find_symbol ge id = Some b /\ f b = Some(b', 0);
   symbols_inject_public: forall id b,
-    Genv.public_symbol se id = true -> 
+    Genv.public_symbol se id = true ->
     Genv.find_symbol ge id = Some b ->
     exists b', Genv.find_symbol tge id = Some b' /\ f b = Some(b', 0);
   info_inject: forall b b' delta gd,
@@ -658,7 +655,7 @@ Remark init_meminj_eq:
   Genv.find_symbol ge id = Some b -> Genv.find_symbol tge id = Some b' ->
   init_meminj se tse b = Some(b', 0).
 Proof.
-  intros. unfold init_meminj. erewrite Genv.find_invert_symbol by eauto. 
+  intros. unfold init_meminj. erewrite Genv.find_invert_symbol by eauto.
   subst tge. cbn in H0. rewrite H0. auto.
 Qed.
 
@@ -677,36 +674,36 @@ Lemma init_meminj_preserves_globals:
   meminj_preserves_globals (init_meminj se tse).
 Proof.
   constructor; intros.
-- unfold init_meminj in H. repeat destr_in H.
+(* - unfold init_meminj in H. repeat destr_in H.
   apply Genv.invert_find_symbol in Heqo.
   apply Genv.genv_vars_eq in Heqo.
-  apply Genv.genv_vars_eq in Heqo0. split; congruence.
+  apply Genv.genv_vars_eq in Heqo0. split; congruence. *)
 - exploit init_meminj_invert; eauto. intros (A & id1 & B & C).
   assert (id1 = id) by (eapply (Genv.genv_vars_inj ge); eauto). subst id1.
   auto.
 - exploit symb_incl; eauto. intros (b & F).
   exists b; split; auto. eapply init_meminj_eq; eauto.
-- exploit symbols_inject_init_public; eauto. 
+- exploit symbols_inject_init_public; eauto.
 - exploit init_meminj_invert; eauto. intros (A & id & B & C).
   exploit info_eq; eauto.
   intros EQ.
-  split; auto. 
+  split; auto.
   cbn. unfold Genv.find_info in EQ. rewrite <- EQ.
   apply H0.
 - exploit init_meminj_invert; eauto. intros (A & id & B & C).
   exploit info_eq; eauto.
   intros EQ.
-  split; auto. 
+  split; auto.
   cbn. unfold Genv.find_info in EQ. rewrite EQ.
   apply H0.
 - exploit transform_find_symbol_1; eauto. intros (b' & F). exists b'; split; auto.
   eapply init_meminj_eq; eauto.
-- exploit init_meminj_invert; eauto. intros (A & id & B & C). 
+- exploit init_meminj_invert; eauto. intros (A & id & B & C).
   unfold tge. rewrite Genv.find_def_spec.
   rewrite (Genv.find_invert_symbol tse id); auto.
   unfold ge in H0. rewrite Genv.find_def_spec in H0.
   destruct (Genv.invert_symbol se b) eqn:INV; try discriminate.
-  rewrite (Genv.find_invert_symbol se id) in INV; auto. 
+  rewrite (Genv.find_invert_symbol se id) in INV; auto.
   inv INV.
   generalize (erase_program_defmap p i).
   rewrite H0. cbn [option_map].
@@ -718,14 +715,14 @@ Proof.
   unfold option_map in TDEF.
   destruct ((prog_defmap tp) ! i) eqn:TDEF'; try discriminate.
   inv TDEF.
-  inv TRANSF. 
+  inv TRANSF.
   rewrite (match_prog_def0 i) in TDEF'.
   destruct (IS.mem i used) eqn:MEM; try discriminate.
   rewrite H0 in TDEF'. inv TDEF'.
   split; auto.
   split; auto.
   inv USED_VALID.
-  intros. 
+  intros.
   apply used_closed0 with i g; eauto.
   apply IS.mem_2; auto.
   erewrite inj_preserved in MEM; eauto. congruence.
@@ -800,20 +797,20 @@ Proof.
     destruct H1 as [b2 INJ]. rewrite H in INJ. congruence.
     destruct (IS.mem i used) eqn:MEM; try discriminate.
     inv USED_VALID.
-    intros. 
+    intros.
     apply used_closed0 with i gd; eauto.
     apply IS.mem_2; eauto.
     erewrite inj_preserved in MEM; eauto. congruence.
 Qed.
 
 (*  generalize init_meminj_preserves_globals.
-  intros PRES. 
+  intros PRES.
   constructor.
   - inv PRES. intros.
-    eapply symbols_inject_4; eauto.    
+    eapply symbols_inject_4; eauto.
     eapply winj_consistent_1; eauto.
     eapply Genv.genv_symb_range; eauto.
-  - inv PRES. intros. 
+  - inv PRES. intros.
     exploit symbols_inject_5; eauto.
     intros (b & FND & INIT).
     exists b; split; auto.
@@ -845,10 +842,10 @@ Lemma globals_symbols_inject:
 Proof.
   intros.
   split; [|split;[|split]]; intros.
-  + unfold ge, tge. cbn. 
+  + unfold ge, tge. cbn.
     rewrite se_public_same. auto.
   + eapply symbols_inject_1; eauto.
-  + exploit symbols_inject_public; eauto. 
+  + exploit symbols_inject_public; eauto.
     intros (b' & FND & INJ).
     eauto.
   + unfold Genv.block_is_volatile.
@@ -921,27 +918,19 @@ Proof.
   apply set_reg_inject; auto.
 Qed.
 
-Inductive astackseq : stackadt -> stackadt -> Prop :=
-  |astackseq_nil : astackseq nil nil
-  |astackseq_cons : forall tl1 tl2 b1 b2 size,
-      astackseq tl1 tl2 ->
-      astackseq (((mk_frame b1 size) :: nil) :: tl1) (((mk_frame b2 size) :: nil) :: tl2).
+Inductive match_astack: nat -> stackadt -> stackadt -> Prop :=
+  | match_astack_nil: forall a1 a2
+      (IHastk: stack_size a1 >= stack_size a2),
+      match_astack O a1 a2
+  | match_astack_cons: forall n tl1 tl2 b1 b2 size
+      (IHastk: match_astack n tl1 tl2),
+      match_astack (S n) (((mk_frame b1 size) :: nil ) :: tl1) (((mk_frame b2 size) :: nil) :: tl2)
+.
 
-Lemma astackseq_nil_refl : forall as1 as2,
-    astackseq as1 as2 ->
-    as1 <> nil <-> as2 <> nil.
-Proof.
-  intros. induction H; eauto. reflexivity.
-  split; congruence.
-Qed.
-
-Lemma astackseq_size : forall as1 as2,
-    astackseq as1 as2 ->
-    stack_size as1 = stack_size as2.
-Proof.
-  intros. induction H; eauto.
-  simpl. unfold frame_size_a. simpl.  lia.
-Qed.
+Remark match_astack_size: forall n a1 a2,
+    match_astack n a1 a2 ->
+    stack_size a1 >= stack_size a2.
+Proof. intros. induction H. auto. simpl. unfold frame_size_a. simpl. lia. Qed.
 
 Inductive match_stacks (j: meminj):
         list stackframe -> list stackframe -> sup -> sup -> Prop :=
@@ -986,7 +975,7 @@ Lemma match_stacks_incr_bound
        Mem.sup_include tbound tbound' -> match_stacks j s ts bound' tbound'.
 Proof.
   intros. inv H. inv H3.
-  econstructor; eauto. rewrite <- H9. econstructor; eauto.
+  econstructor; eauto. rewrite <- H. econstructor; eauto.
   econstructor; eauto.
 Qed.
 
@@ -996,11 +985,11 @@ Lemma match_stacks_match_stbls:
     match_stacks j s ts sp tsp ->
     Genv.match_stbls j se tse.
 Proof.
-  induction 2; eauto. 
+  induction 2; eauto.
   generalize (CKLR.match_stbls_acc inj). cbn.
   intros MONO.
-  repeat red in MONO. 
-  generalize (MONO _ _ H1 se tse). intros SUB. 
+  repeat red in MONO.
+  generalize (MONO _ _ H1 se tse). intros SUB.
   apply SUB.
   apply H.
 Qed.
@@ -1033,18 +1022,11 @@ Proof.
   assert (SAME': forall b b' delta, sup_In b' (Genv.genv_sup tge) ->
                                j' b = Some(b', delta) -> j b = Some (b', delta)).
   { intros. destruct (j b) as [[b1 delta1] | ] eqn: J.
-<<<<<<< HEAD
     exploit INCR; eauto. congruence.
     exploit SEP; eauto. intros [A B].
     exfalso. apply B. apply BND2; eauto. }
-  constructor; intros.  
-=======
-    exploit H; eauto. congruence.
-    exploit H3; eauto. intros [A B].
-    apply H2 in H4. congruence. }
-  constructor; auto.  constructor; intros.
-  + exploit symbols_inject_0; eauto.
->>>>>>> origin/StackAware-new
+  constructor; intros.
+  (* + exploit symbols_inject_0; eauto. *)
   + exploit symbols_inject_1; eauto. apply SAME; auto.
     eapply Genv.genv_symb_range; eauto.
   + exploit symbols_inject_3; eauto. intros (b & A & B).
@@ -1063,9 +1045,9 @@ Qed.
 
 
 Lemma match_stacks_incr_aux:
-  forall j bound tbound s ts, 
+  forall j bound tbound s ts,
     match_stacks j s ts bound tbound ->
-    forall j' bound' tbound', 
+    forall j' bound' tbound',
       inj_incr (injw j bound tbound) (injw j' bound' tbound') ->
       match_stacks j' s ts bound' tbound'.
 Proof.
@@ -1079,20 +1061,20 @@ Proof.
 - inv H0. econstructor; eauto.
   + apply IHmatch_stacks; auto.
     ++ constructor; auto; try lia.
-       intro. intros. exploit H8; eauto.
+       intro. intros. exploit DISJOINT; eauto.
        intros (BND1 & BND2). split.
-       intro. apply BND1. apply BELOW. right. eauto.
-       intro. apply BND2. apply TBELOW. right. eauto.
+       intro. apply BND1. apply BELOW. eapply Mem.sup_include_incr. auto.
+       intro. apply BND2. apply TBELOW. eapply Mem.sup_include_incr. auto.
   + eapply regset_inject_incr; eauto.
 Qed.
 
 Lemma match_stacks_incr:
-  forall j j' bound bound' tbound tbound' s ts, 
+  forall j j' bound bound' tbound tbound' s ts,
     inj_incr (injw j bound tbound) (injw j' bound' tbound') ->
     match_stacks j s ts bound tbound ->
     match_stacks j' s ts bound' tbound'.
 Proof.
-  intros. 
+  intros.
   apply match_stacks_incr_aux with j bound tbound; auto.
 Qed.
 
@@ -1104,7 +1086,7 @@ Lemma match_stacks_bound:
 Proof.
   induction 1; intros.
 - econstructor; eauto with mem.
-  + inv H0. 
+  + inv H0.
     constructor; eauto with mem.
 - econstructor; eauto.
 Qed.
@@ -1119,37 +1101,40 @@ Inductive match_states: state -> state -> Prop :=
          (SPINJ: j sp = Some(tsp, 0))
          (REGINJ: regset_inject j rs trs)
          (MEMINJ: Mem.inject j m tm)
-         (MASTK: astackseq (Mem.astack (Mem.support m)) (Mem.astack (Mem.support tm)))
+         (INJG: meminj_global j)
+         (ASTK: match_astack (S (length s)) (Mem.astack (Mem.support m)) (Mem.astack (Mem.support tm)))
          (SUPINC: Mem.sup_include sps (Mem.support m))
          (TSUPINC: Mem.sup_include tsps (Mem.support tm)),
       match_states (State s f (Vptr sp Ptrofs.zero) pc rs m)
                    (State ts f (Vptr tsp Ptrofs.zero) pc trs tm)
-<<<<<<< HEAD
-  | match_states_call: forall s vf tvf fd args m ts targs tm j
-=======
-  | match_states_call: forall s fd args m ts targs tm j id
->>>>>>> origin/StackAware-new
+  | match_states_call: forall s vf tvf fd args m ts targs tm j id
          (STACKS: match_stacks j s ts (Mem.support m) (Mem.support tm))
          (FUN: Genv.find_funct ge vf = Some fd)
          (FUNINJ: Val.inject j vf tvf)
          (KEPT: forall id, ref_fundef fd id -> kept id)
          (ARGINJ: Val.inject_list j args targs)
-         (MASTK: astackseq (Mem.astack (Mem.support m)) (Mem.astack (Mem.support tm)))
-         (MEMINJ: Mem.inject j m tm),
-<<<<<<< HEAD
-      match_states (Callstate s vf args m)
-                   (Callstate ts tvf targs tm)
-=======
-      match_states (Callstate s fd args m id)
-                   (Callstate ts fd targs tm id)
->>>>>>> origin/StackAware-new
+         (ASTK: match_astack (length s) (Mem.astack (Mem.support m)) (Mem.astack (Mem.support tm)))
+         (MEMINJ: Mem.inject j m tm)
+         (INJG: meminj_global j),
+      match_states (Callstate s vf args m id)
+                   (Callstate ts tvf targs tm id)
   | match_states_return: forall s res m ts tres tm j
          (STACKS: match_stacks j s ts (Mem.support m) (Mem.support tm))
          (RESINJ: Val.inject j res tres)
-         (MASTK: astackseq (Mem.astack (Mem.support m)) (Mem.astack (Mem.support tm)))
-         (MEMINJ: Mem.inject j m tm),
+         (ASTK: match_astack (length s) (Mem.astack (Mem.support m)) (Mem.astack (Mem.support tm)))
+         (MEMINJ: Mem.inject j m tm)
+         (INJG: meminj_global j),
       match_states (Returnstate s res m)
         (Returnstate ts tres tm).
+
+Ltac injg H :=
+  match type of H with
+  | ?j ?g = Some ?x =>
+      match goal with
+      | INJG: meminj_global j |- _ =>
+          apply INJG in H as []; subst; auto
+      end
+  end.
 
 Lemma external_call_inject:
   forall ef vargs m1 t vres m2 f m1' vargs',
@@ -1163,15 +1148,15 @@ Lemma external_call_inject:
     /\ Mem.inject f' m2 m2'
     /\ Mem.unchanged_on (loc_unmapped f) m1 m2
     /\ Mem.unchanged_on (loc_out_of_reach f m1) m1' m2'
+    /\ Mem.astack (Mem.support m1) = Mem.astack (Mem.support m2)
+    /\ Mem.astack (Mem.support m1') = Mem.astack (Mem.support m2')
     /\ inject_incr f f'
+    /\ incr_without_glob f f'
     /\ inject_separated f f' m1 m1'.
 Proof.
   intros.
   exploit external_call_mem_inject_gen'; eauto.
   apply globals_symbols_inject; auto.
-  intros (f' & vres' & m2' & A & B & C & D & E & F & G & I).
-  exists f',vres',m2'. split. auto. split. auto. split. auto.
-  split. auto. split; auto.
 Qed.
 
 Lemma find_function_inject:
@@ -1191,7 +1176,7 @@ Proof.
   generalize (defs_inject _ PRES _ _ _ _ H1 FIND); eauto.
   intros (FDEF & D' & KEPTS). subst.
   cbn.
-  rewrite Ptrofs.add_zero_l. 
+  rewrite Ptrofs.add_zero_l.
   unfold Ptrofs.zero.
   destruct Ptrofs.eq_dec; try congruence.
   rewrite Genv.find_funct_ptr_iff.
@@ -1207,8 +1192,8 @@ Proof.
   - auto.
   - unfold Genv.symbol_address.
     destruct (Genv.find_symbol se id) as [b|] eqn:FS; auto.
-    exploit symbols_inject_2; eauto. intros (tb & P & Q). 
-    cbn in P. rewrite P. 
+    exploit symbols_inject_2; eauto. intros (tb & P & Q).
+    cbn in P. rewrite P.
     econstructor; eauto.
 Qed.
 
@@ -1217,7 +1202,7 @@ Lemma find_function_inject_ros:
   meminj_preserves_globals j ->
   Genv.find_funct ge (ros_address ge ros rs) = Some fd ->
   match ros with inl r => regset_inject j rs trs | inr id => kept id end ->
-  Genv.find_funct tge (ros_address tge ros trs) = Some fd /\ 
+  Genv.find_funct tge (ros_address tge ros trs) = Some fd /\
   (forall id, ref_fundef fd id -> kept id).
 Proof.
   intros j ros rs fd trs PRES FIND ROS.
@@ -1249,7 +1234,7 @@ Proof.
   intros (v' & A & B). exists v'; auto with barg.
 - econstructor; split; eauto with barg. simpl. econstructor; eauto. rewrite Ptrofs.add_zero; auto.
 - assert (Val.inject j (Genv.symbol_address ge id ofs) (Genv.symbol_address tge id ofs)).
-  { unfold Genv.symbol_address. 
+  { unfold Genv.symbol_address.
     destruct (Genv.find_symbol ge id) as [b|] eqn:FS; auto.
     exploit symbols_inject_2; eauto. intros (b' & A & B). rewrite A.
     econstructor; eauto. rewrite Ptrofs.add_zero; auto. }
@@ -1292,21 +1277,18 @@ Qed.
 Lemma ros_is_ident_transf:
     forall ros rs trs j id fd,
       ros_is_ident ros rs id ->
-      find_function ge ros rs = Some fd ->
-      meminj_preserves_globals j ->
+      let vf := ros_address ge ros rs in
+      Genv.find_funct ge vf = Some fd ->
+      meminj_global j ->
       regset_inject j rs trs ->
       ros_is_ident ros trs id.
 Proof.
   intros.
-  destruct ros; simpl in *.  generalize (H2 r).
+  destruct ros; simpl in *. generalize (H2 r).
   intro. inv H3; (try congruence).
   rewrite H in H4. inv H4.
-  rewrite H in H0. simpl in H0.
-  destr_in H0. subst. unfold Genv.find_funct_ptr in H0.
-  destr_in H0. inv H0. inv H1.
-  exploit symbols_inject_4; eauto. eapply Genv.genv_defs_range; eauto.
-  intros [C D]. subst. intros. eauto.
-  eauto.
+  injg H6.
+  auto.
 Qed.
 
 Theorem step_simulation:
@@ -1367,68 +1349,27 @@ Proof.
   destruct A as (ta & B & C).
   exploit Mem.storev_mapped_inject; eauto. intros (tm' & D & E).
   econstructor; split. eapply exec_Istore; eauto.
-<<<<<<< HEAD
-  econstructor; eauto. erewrite <- Mem.support_storev; eauto.
+  econstructor; eauto.
+  erewrite <- Mem.support_storev; eauto.
+  erewrite <- (Mem.support_storev _ _ _ _ tm'); eauto.
+  erewrite <- Mem.support_storev; eauto.
   erewrite <- Mem.support_storev; eauto.
 
-=======
-  econstructor;
-  try (rewrite <- (Mem.support_storev _ _ _ _ _ H1)); eauto.
-  rewrite <- (Mem.support_storev _ _ _ _ _ D). auto.
-  rewrite <- (Mem.support_storev _ _ _ _ _ D). auto.
->>>>>>> origin/StackAware-new
 - (* call *)
   exploit find_function_inject_ros.
   eapply match_stacks_preserves_globals; eauto. eauto.
   destruct ros as [r|id']. eauto. apply KEPT. red. econstructor; econstructor; split; eauto. simpl; auto.
   intros (A & B).
   econstructor; split. eapply exec_Icall; eauto.
-  eapply ros_is_ident_transf; eauto. eapply match_stacks_preserves_globals; eauto.
+  eapply ros_is_ident_transf; eauto.
   econstructor; eauto.
-<<<<<<< HEAD
   + econstructor; eauto.
-    intro. intro. apply Mem.sup_incr_in in H1. destruct H1.
+    intro. intro. apply Mem.sup_incr_in in H2. destruct H2.
     change (Mem.valid_block m b). subst b. eapply Mem.valid_block_inject_1; eauto.
     apply SUPINC; eauto.
-    intro. intro. apply Mem.sup_incr_in in H1. destruct H1.
+    intro. intro. apply Mem.sup_incr_in in H2. destruct H2.
     change (Mem.valid_block tm b). subst b. eapply Mem.valid_block_inject_2; eauto.
     apply TSUPINC; eauto.
-  + subst vf.
-    unfold ros_address. 
-    destruct ros; eauto.
-    eapply symbol_address_inject; eauto.
-    eapply match_stacks_preserves_globals; eauto.
-    apply KEPT. red. econstructor; econstructor; split; eauto. simpl; auto.
-  + apply regs_inject; auto.
-=======
-  econstructor; eauto.
-  intro. intro. apply Mem.sup_incr_in in H2. destruct H2.
-  change (Mem.valid_block m b). subst b. eapply Mem.valid_block_inject_1;eauto. apply SUPINC; auto.
-  intro. intro. apply Mem.sup_incr_in in H2. destruct H2.
-  change (Mem.valid_block tm b). subst b. eapply Mem.valid_block_inject_2;eauto. apply TSUPINC; auto.
-  apply regs_inject; auto.
->>>>>>> origin/StackAware-new
-
-    
-- (* tailcall *)
-  exploit find_function_inject_ros.
-  eapply match_stacks_preserves_globals; eauto. eauto.
-  destruct ros as [r|id']. eauto. apply KEPT. red. econstructor; econstructor; split; eauto. simpl; auto.
-  intros (A & B).
-  exploit Mem.free_parallel_inject; eauto. rewrite ! Z.add_0_r. intros (tm' & C & D).
-  apply Mem.support_free in C as SUPF. apply Mem.support_free in H3 as SUPF'.
-  exploit Mem.pop_stage_parallel_inject; eauto. rewrite SUPF. apply astackseq_nil_refl in MASTK.
-  rewrite <- MASTK. rewrite <- SUPF'.            
-  eapply Mem.pop_stage_nonempty; eauto.
-  intros (tm''' & G & I).
-  econstructor; split.
-  eapply exec_Itailcall; eauto.
-  eapply ros_is_ident_transf; eauto. eapply match_stacks_preserves_globals; eauto.
-  econstructor; eauto.
-<<<<<<< HEAD
-  + apply match_stacks_bound with sps tsps; auto.
-    erewrite Mem.support_free; eauto.
-    erewrite Mem.support_free; eauto.
   + subst vf.
     unfold ros_address.
     destruct ros; eauto.
@@ -1437,19 +1378,41 @@ Proof.
     apply KEPT. red. econstructor; econstructor; split; eauto. simpl; auto.
   + apply regs_inject; auto.
 
-=======
-  apply match_stacks_bound with sps tsps; auto.
-  eapply Mem.sup_include_trans; eauto.
-  erewrite <- Mem.support_free; eauto.
-  intro. eapply Mem.support_pop_stage_1 in H4. apply H4.
-  eapply Mem.sup_include_trans; eauto.
-  erewrite <- Mem.support_free; eauto.
-  intro. eapply Mem.support_pop_stage_1 in G. apply G.
-  apply regs_inject; auto.
-  apply Mem.astack_pop_stage in H4. destruct H4. apply Mem.astack_pop_stage in G.
-  destruct G. rewrite <- SUPF', H2 in MASTK. rewrite <- SUPF, H4 in MASTK.
-  inv MASTK. eauto.
->>>>>>> origin/StackAware-new
+- (* tailcall *)
+  exploit find_function_inject_ros.
+  eapply match_stacks_preserves_globals; eauto. eauto.
+  destruct ros as [r|id']. eauto. apply KEPT. red. econstructor; econstructor; split; eauto. simpl; auto.
+  intros (A & B).
+  exploit Mem.free_parallel_inject; eauto. rewrite ! Z.add_0_r. intros (tm' & C & D).
+  apply Mem.support_free in C as SUPF. apply Mem.support_free in H3 as SUPF'.
+  exploit Mem.pop_stage_parallel_inject; eauto.
+    rewrite SUPF. inv ASTK. congruence.
+  intros (tm''' & G & I).
+  econstructor; split.
+  eapply exec_Itailcall; eauto.
+  eapply ros_is_ident_transf; eauto.
+  econstructor; eauto.
+  + apply match_stacks_bound with sps tsps; auto.
+    red. intros.
+    rewrite <- Mem.support_pop_stage_1. 2:eauto.
+    erewrite Mem.support_free; eauto.
+    red. intros.
+    rewrite <- Mem.support_pop_stage_1. 2:eauto.
+    erewrite Mem.support_free; eauto.
+  + subst vf.
+    unfold ros_address.
+    destruct ros; eauto.
+    eapply symbol_address_inject; eauto.
+    eapply match_stacks_preserves_globals; eauto.
+    apply KEPT. red. econstructor; econstructor; split; eauto. simpl; auto.
+  + apply regs_inject; auto.
+  + inv ASTK.
+    erewrite <- Mem.support_free in H6; eauto.
+    erewrite <- Mem.support_free in H7; eauto.
+    apply Mem.astack_pop_stage in H4 as [hd1 POP1]. rewrite POP1 in H6. inv H6.
+    apply Mem.astack_pop_stage in G as [hd2 POP2]. rewrite POP2 in H7. inv H7.
+    auto.
+
 - (* builtin *)
   exploit eval_builtin_args_inject; eauto.
   eapply match_stacks_preserves_globals; eauto.
@@ -1457,32 +1420,21 @@ Proof.
   intros (vargs' & P & Q).
   exploit external_call_inject; eauto.
   eapply match_stacks_preserves_globals; eauto.
-  intros (j' & tv & tm' & A & B & C & D & E & F & G).
+  intros (j' & tv & tm' & A & B & C & D & E & F & G & I & J & K).
   econstructor; split.
   eapply exec_Ibuiltin; eauto.
   eapply match_states_regular with (j := j'); eauto.
-<<<<<<< HEAD
   + apply match_stacks_incr with j sps tsps; eauto.
     constructor; auto.
-    intro. intros. exploit G; eauto. intros [U V]. split.
+    intro. intros. exploit K; eauto. intros [U V]. split.
     intro. apply U. apply SUPINC; eauto.
     intro. apply V. apply TSUPINC; eauto.
   + apply set_res_inject; auto. apply regset_inject_incr with j; auto.
+  + eapply meminj_global_incr; eauto.
+  + congruence.
   + inversion D. eauto with mem.
   + inversion E. eauto with mem.
 
-=======
-  apply match_stacks_incr with j; auto.
-  intros. exploit G; eauto. intros [U V].
-  split.
-  intro. apply SUPINC in H4. apply U. auto.
-  intro. apply TSUPINC in H4. apply V. auto.
-  apply set_res_inject; auto. apply regset_inject_incr with j; auto.
-  apply external_call_astack in H1. apply external_call_astack in A.
-  congruence.
-  eapply Mem.sup_include_trans. eauto. eapply Mem.unchanged_on_support;eauto.
-  eapply Mem.sup_include_trans. eauto. eapply Mem.unchanged_on_support;eauto.
->>>>>>> origin/StackAware-new
 - (* cond *)
   assert (C: eval_condition cond trs##args tm = Some b).
   { eapply eval_condition_inject; eauto. apply regs_inject; auto. }
@@ -1499,81 +1451,76 @@ Proof.
 - (* return *)
   exploit Mem.free_parallel_inject; eauto. rewrite ! Z.add_0_r. intros (tm' & C & D).
   apply Mem.support_free in H0 as SUPF. apply Mem.support_free in C as SUPF'.
-  exploit Mem.pop_stage_parallel_inject; eauto.
-  apply Mem.pop_stage_nonempty in H1.
-  apply astackseq_nil_refl in MASTK. rewrite SUPF'. apply MASTK. rewrite <- SUPF. eauto.
-  intros (tm''' & G & I).
+  exploit Mem.pop_stage_parallel_inject; eauto. inv ASTK. congruence. intros (tm''' & G & I).
   econstructor; split.
   eapply exec_Ireturn; eauto.
   econstructor; subst; eauto.
-  apply match_stacks_bound with sps tsps; auto.
-  eapply Mem.sup_include_trans; eauto.
-  erewrite <- Mem.support_free; eauto.
-  intro. eapply Mem.support_pop_stage_1 in H1. apply H1.
-  eapply Mem.sup_include_trans; eauto.
-  erewrite <- Mem.support_free; eauto.
-  intro. eapply Mem.support_pop_stage_1 in G. apply G.
-  destruct or; simpl; auto.
-  apply Mem.astack_pop_stage in H1. destruct H1. apply Mem.astack_pop_stage in G.
-  destruct G. rewrite <- SUPF', H2, <- SUPF, H1 in MASTK. inv MASTK. eauto.
+  + apply match_stacks_bound with sps tsps; auto.
+    red. intros.
+    rewrite <- Mem.support_pop_stage_1. 2:eauto.
+    erewrite Mem.support_free; eauto.
+    red. intros.
+    rewrite <- Mem.support_pop_stage_1. 2:eauto.
+    erewrite Mem.support_free; eauto.
+  + destruct or; simpl; auto.
+  + inv ASTK.
+    erewrite <- Mem.support_free in H4; eauto.
+    erewrite <- Mem.support_free in H5; eauto.
+    apply Mem.astack_pop_stage in H1 as [hd1 POP1]. rewrite POP1 in H4. inv H4.
+    apply Mem.astack_pop_stage in G as [hd2 POP2]. rewrite POP2 in H5. inv H5.
+    auto.
 - (* internal function *)
   exploit Mem.alloc_parallel_inject. eauto. eauto. apply Z.le_refl. apply Z.le_refl.
-  intros (j' & tm'' & tstk & C & D & E & F & G).
+  intros (j' & tm'' & tstk & C & D & E & F & G & I).
   apply Mem.astack_alloc in H as ASTKA.
-  apply Mem.astack_alloc in C as ASTKA'. 
+  apply Mem.astack_alloc in C as ASTKA'.
   exploit Mem.push_stage_inject. eauto. intro.
-  exploit Mem.record_frame_parallel_inject; eauto. simpl. congruence.
-  simpl. rewrite ASTKA', ASTKA. apply astackseq_size in MASTK. lia.
-  intros (tm''' & I & J).
+  exploit Mem.record_frame_parallel_inject; eauto.
+    simpl. congruence.
+    simpl. rewrite ASTKA, ASTKA'. apply match_astack_size in ASTK. lia.
+  intros (tm''' & J & K).
   assert (STK: stk = Mem.nextblock m) by (eapply Mem.alloc_result; eauto).
   assert (TSTK: tstk = Mem.nextblock tm) by (eapply Mem.alloc_result; eauto).
   assert (STACKS': match_stacks j' s ts (Mem.support m) (Mem.support tm)).
-<<<<<<< HEAD
-  { 
+  {
     apply match_stacks_incr with j (Mem.support m) (Mem.support tm); auto.
     constructor; auto; try lia.
     intro. intros. destruct (eq_block b stk).
-    subst b. rewrite F in H1; inv H1.
+    subst b. rewrite G in H3. inv H3.
     split; apply freshness.
-    rewrite G in H1 by auto. congruence. }
-=======
-  {
-    apply match_stacks_incr with j; auto.
-    intros. destruct (eq_block b1 stk).
-    subst b1. rewrite F in H3; inv H3. split. apply freshness.
-    apply freshness.
-    rewrite G in H3 by auto. congruence. }
->>>>>>> origin/StackAware-new
+    rewrite I in H3 by auto. congruence. }
   econstructor; split.
   rewrite FIND in FUN. inv FUN.
   eapply exec_function_internal; eauto.
   eapply find_function_inject; eauto.
   generalize (match_stacks_preserves_globals _ _ _ _ _ STACKS).
-  auto. 
+  auto.
   subst.
   eapply match_states_regular with (j := j'); eauto.
-<<<<<<< HEAD
   + reflexivity.
   + reflexivity.
-  + intros id REF. rewrite FIND in FUN. inv FUN. auto.
+  + intros id' REF. rewrite FIND in FUN. inv FUN. auto.
   + apply init_regs_inject; auto. apply val_inject_list_incr with j; auto.
-  + rewrite (Mem.support_alloc _ _ _ _ _  H). apply Mem.sup_incr_in2.
-  + rewrite (Mem.support_alloc _ _ _ _ _  C). apply Mem.sup_incr_in2.
-=======
-  apply init_regs_inject; auto. apply val_inject_list_incr with j; auto.
-  apply Mem.astack_record_frame in H0. apply Mem.astack_record_frame in I.
-  destruct H0 as [a [b [c d]]]. destruct I as [e[f'[g h]]]. simpl in *.
-  rewrite d,h. inv g. inv c. econstructor. rewrite ASTKA, ASTKA'. auto.
-  eapply Mem.sup_include_trans. 2: { intro; eapply Mem.support_record_frame_1 in H0; apply H0; eauto. } simpl.
-  rewrite Mem.support_alloc with m 0 (fn_stacksize f) m' stk. apply Mem.sup_incr_in2. auto.
-  eapply Mem.sup_include_trans. 2: {intro; eapply Mem.support_record_frame_1 in I. apply I; eauto. } simpl.
-  rewrite Mem.support_alloc with tm 0 (fn_stacksize f) tm'' tstk. apply Mem.sup_incr_in2. auto.
->>>>>>> origin/StackAware-new
+  + eapply meminj_global_incr; eauto.
+  + apply Mem.astack_record_frame in H0 as (hd & tl & EQ1 & EQ2). simpl in EQ1. inv EQ1.
+    apply Mem.astack_record_frame in J as (hd' & tl' & EQ1' & EQ2'). simpl in EQ1'. inv EQ1'.
+    rewrite EQ2, EQ2'. constructor.
+    erewrite Mem.support_alloc; eauto.
+    erewrite (Mem.support_alloc _ _ _ tm''); eauto.
+    simpl. auto.
+  + red. intros.
+    erewrite <- Mem.support_record_frame_1. 2:eauto.
+    erewrite <- Mem.support_push_stage_1. 2:eauto.
+    erewrite Mem.support_alloc; eauto. apply Mem.sup_include_incr. auto.
+  + red. intros.
+    erewrite <- Mem.support_record_frame_1. 2:eauto.
+    erewrite <- Mem.support_push_stage_1. 2:eauto.
+    erewrite Mem.support_alloc; eauto. apply Mem.sup_include_incr. auto.
 
 - (* external function *)
   exploit external_call_inject; eauto.
   eapply match_stacks_preserves_globals; eauto.
-  intros (j' & tres & tm' & A & B & C & D & E & F & G).
+  intros (j' & tres & tm' & A & B & C & D & E & F & G & I & J & K).
   econstructor; split.
   rewrite FIND in FUN. inv FUN.
   eapply exec_function_external; eauto.
@@ -1582,208 +1529,14 @@ Proof.
   auto.
   eapply match_states_return with (j := j'); eauto.
   apply match_stacks_bound with (Mem.support m) (Mem.support tm).
-<<<<<<< HEAD
-  apply match_stacks_incr 
+  apply match_stacks_incr
     with j (Mem.support m) (Mem.support tm); auto.
-  inversion D. eauto. inversion E. eauto.
-=======
-  apply match_stacks_incr with j; auto.
-  eapply external_call_support; eauto.
-  eapply external_call_support; eauto.
-  apply external_call_astack in H. apply external_call_astack in A.
-  congruence.
->>>>>>> origin/StackAware-new
+  inversion D. eauto. inversion E. eauto. congruence. eapply meminj_global_incr; eauto.
 
 - (* return *)
   inv STACKS. econstructor; split.
   eapply exec_return.
   econstructor; eauto. apply set_reg_inject; auto.
-<<<<<<< HEAD
-=======
-  intro. intro. apply BELOW. apply Mem.sup_incr_in2. auto.
-  intro. intro. apply TBELOW. apply Mem.sup_incr_in2. auto.
-Qed.
-
-(** Relating initial memory states *)
-
-(*
-Remark genv_find_def_exists:
-  forall (F V: Type) (p: AST.program F V) b,
-  Plt b (Genv.genv_next (Genv.globalenv p)) ->
-  exists gd, Genv.find_def (Genv.globalenv p) b = Some gd.
-Proof.
-  intros until b.
-  set (P := fun (g: Genv.t F V) =>
-        Plt b (Genv.genv_next g) -> exists gd, (Genv.genv_defs g)!b = Some gd).
-  assert (forall l g, P g -> P (Genv.add_globals g l)).
-  { induction l as [ | [id1 g1] l]; simpl; intros.
-  - auto.
-  - apply IHl. unfold Genv.add_global, P; simpl. intros LT. apply Plt_succ_inv in LT. destruct LT.
-  + rewrite PTree.gso. apply H; auto. apply Plt_ne; auto.
-  + rewrite H0. rewrite PTree.gss. exists g1; auto. }
-  apply H. red; simpl; intros. exfalso; extlia.
-Qed.
-*)
-
-Lemma init_meminj_invert_strong:
-  forall b b' delta,
-  init_meminj b = Some(b', delta) ->
-  delta = 0 /\
-  exists id gd,
-     Genv.find_symbol ge id = Some b
-  /\ Genv.find_symbol tge id = Some b'
-  /\ Genv.find_def ge b = Some gd
-  /\ Genv.find_def tge b' = Some gd
-  /\ (forall i, ref_def gd i -> kept i).
-Proof.
-  intros. exploit init_meminj_invert; eauto. intros (A & id & B & C).
-  assert (exists gd, (prog_defmap p)!id = Some gd).
-  { apply prog_defmap_dom. eapply Genv.find_symbol_inversion; eauto. }
-  destruct H0 as [gd DM]. rewrite Genv.find_def_symbol in DM.
-  destruct DM as (b'' & P & Q). fold ge in P. rewrite P in B; inv B.
-  fold ge in Q. exploit defs_inject. apply init_meminj_preserves_globals.
-  eauto. eauto. intros (X & _ & Y).
-  split. auto. exists id, gd; auto.
-Qed.
-
-Section INIT_MEM.
-
-Variables m tm: mem.
-Hypothesis IM: Genv.init_mem p = Some m.
-Hypothesis TIM: Genv.init_mem tp = Some tm.
-
-Lemma bytes_of_init_inject:
-  forall il,
-  (forall id, ref_init il id -> kept id) ->
-  list_forall2 (memval_inject init_meminj) (Genv.bytes_of_init_data_list ge il) (Genv.bytes_of_init_data_list tge il).
-Proof.
-  induction il as [ | i1 il]; simpl; intros.
-- constructor.
-- apply list_forall2_app.
-+ destruct i1; simpl; try (apply inj_bytes_inject).
-  induction (Z.to_nat z); simpl; constructor. constructor. auto.
-  destruct (Genv.find_symbol ge i) as [b|] eqn:FS.
-  assert (kept i). { apply H. red. exists i0; auto with coqlib. }
-  exploit symbols_inject_2. apply init_meminj_preserves_globals. eauto. eauto.
-  intros (b' & A & B). rewrite A. apply inj_value_inject.
-  econstructor; eauto. symmetry; apply Ptrofs.add_zero.
-  destruct (Genv.find_symbol tge i) as [b'|] eqn:FS'.
-  exploit symbols_inject_3. apply init_meminj_preserves_globals. eauto.
-  intros (b & A & B). congruence.
-  apply repeat_Undef_inject_self.
-+ apply IHil. intros id [ofs IN]. apply H. exists ofs; auto with coqlib.
-Qed.
-
-Lemma Mem_getN_forall2:
-  forall (P: memval -> memval -> Prop) c1 c2 i n p,
-  list_forall2 P (Mem.getN n p c1) (Mem.getN n p c2) ->
-  p <= i -> i < p + Z.of_nat n ->
-  P (ZMap.get i c1) (ZMap.get i c2).
-Proof.
-  induction n; simpl Mem.getN; intros.
-- simpl in H1. extlia.
-- inv H. rewrite Nat2Z.inj_succ in H1. destruct (zeq i p0).
-+ congruence.
-+ apply IHn with (p0 + 1); auto. lia. lia.
-Qed.
-
-Lemma init_mem_inj_1:
-  Mem.mem_inj init_meminj m tm.
-Proof.
-  intros; constructor; intros.
-- exploit init_meminj_invert_strong; eauto. intros (A & id & gd & B & C & D & E & F).
-  exploit (Genv.init_mem_characterization_gen p); eauto.
-  exploit (Genv.init_mem_characterization_gen tp); eauto.
-  destruct gd as [f|v].
-+ intros (P2 & Q2) (P1 & Q1).
-  apply Q1 in H0. destruct H0. subst.
-  apply Mem.perm_cur. auto.
-+ intros (P2 & Q2 & R2 & S2) (P1 & Q1 & R1 & S1).
-  apply Q1 in H0. destruct H0. subst.
-  apply Mem.perm_cur. eapply Mem.perm_implies; eauto.
-  apply P2. lia.
-- exploit init_meminj_invert; eauto. intros (A & id & B & C).
-  subst delta. apply Z.divide_0_r.
-- exploit init_meminj_invert_strong; eauto. intros (A & id & gd & B & C & D & E & F).
-  exploit (Genv.init_mem_characterization_gen p); eauto.
-  exploit (Genv.init_mem_characterization_gen tp); eauto.
-  destruct gd as [f|v].
-+ intros (P2 & Q2) (P1 & Q1).
-  apply Q1 in H0. destruct H0; discriminate.
-+ intros (P2 & Q2 & R2 & S2) (P1 & Q1 & R1 & S1).
-  apply Q1 in H0. destruct H0.
-  assert (NO: gvar_volatile v = false).
-  { unfold Genv.perm_globvar in H1. destruct (gvar_volatile v); auto. inv H1. }
-Local Transparent Mem.loadbytes.
-  generalize (S1 NO). unfold Mem.loadbytes. destruct Mem.range_perm_dec; intros E1; inv E1.
-  generalize (S2 NO). unfold Mem.loadbytes. destruct Mem.range_perm_dec; intros E2; inv E2.
-  rewrite Z.add_0_r.
-  apply Mem_getN_forall2 with (p := 0) (n := Z.to_nat (init_data_list_size (gvar_init v))).
-  rewrite H3, H4. apply bytes_of_init_inject. auto.
-  lia.
-  rewrite Z2Nat.id by (apply Z.ge_le; apply init_data_list_size_pos). lia.
-Qed.
-
-Lemma init_mem_inj_2:
-  Mem.inject init_meminj m tm.
-Proof.
-  constructor; intros.
-- apply init_mem_inj_1.
-- destruct (init_meminj b) as [[b' delta]|] eqn:INJ; auto.
-  elim H. exploit init_meminj_invert; eauto. intros (A & id & B & C).
-  eapply Genv.find_symbol_not_fresh; eauto.
-- exploit init_meminj_invert; eauto. intros (A & id & B & C).
-  eapply Genv.find_symbol_not_fresh; eauto.
-- red; intros.
-  exploit init_meminj_invert. eexact H0. intros (A1 & id1 & B1 & C1).
-  exploit init_meminj_invert. eexact H1. intros (A2 & id2 & B2 & C2).
-  destruct (ident_eq id1 id2). congruence. left; eapply Genv.global_addresses_distinct; eauto.
-- exploit init_meminj_invert; eauto. intros (A & id & B & C). subst delta.
-  split. lia. generalize (Ptrofs.unsigned_range_2 ofs). lia.
-- exploit init_meminj_invert_strong; eauto. intros (A & id & gd & B & C & D & E & F).
-  exploit (Genv.init_mem_characterization_gen p); eauto.
-  exploit (Genv.init_mem_characterization_gen tp); eauto.
-  destruct gd as [f|v].
-+ intros (P2 & Q2) (P1 & Q1).
-  apply Q2 in H0. destruct H0. subst. replace ofs with 0 by lia.
-  left; apply Mem.perm_cur; auto.
-+ intros (P2 & Q2 & R2 & S2) (P1 & Q1 & R1 & S1).
-  apply Q2 in H0. destruct H0. subst.
-  left. apply Mem.perm_cur. eapply Mem.perm_implies; eauto.
-  apply P1. lia.
-Qed.
-
-End INIT_MEM.
-
-Lemma init_mem_exists:
-  forall m, Genv.init_mem p = Some m ->
-  exists tm, Genv.init_mem tp = Some tm.
-Proof.
-  intros. apply Genv.init_mem_exists.
-  intros.
-  assert (P: (prog_defmap tp)!id = Some (Gvar v)).
-  { eapply prog_defmap_norepet; eauto. eapply match_prog_unique; eauto. }
-  rewrite (match_prog_def _ _ _ TRANSF) in P. destruct (IS.mem id used) eqn:U; try discriminate.
-  exploit Genv.init_mem_inversion; eauto. apply in_prog_defmap; eauto. intros [AL FV].
-  split. auto.
-  intros. exploit FV; eauto. intros (b & FS).
-  apply transform_find_symbol_1 with b; auto.
-  apply kept_closed with id (Gvar v).
-  apply IS.mem_2; auto. auto. red. red. exists o; auto.
-Qed.
-
-Theorem init_mem_inject:
-  forall m,
-  Genv.init_mem p = Some m ->
-  exists tm, Genv.init_mem tp = Some tm /\ Mem.inject init_meminj m tm /\ meminj_preserves_globals init_meminj.
-Proof.
-  intros.
-  exploit init_mem_exists; eauto. intros [tm INIT].
-  exists tm.
-  split. auto.
-  split. eapply init_mem_inj_2; eauto.
-  apply init_meminj_preserves_globals.
->>>>>>> origin/StackAware-new
 Qed.
 
 Lemma transf_initial_states:
@@ -1792,59 +1545,27 @@ Lemma transf_initial_states:
   forall S, initial_state ge q1 S ->
   exists R, initial_state tge q2 R /\ match_states S R.
 Proof.
-<<<<<<< HEAD
   intros q1 q2 MQUERY S INIT_STATE.
   inv MQUERY. inv INIT_STATE.
   cbn in *.
   generalize inj_world_preserves_globals.
   intros PRES.
-  eexists; split. 
+  eexists; split.
   - constructor.
     generalize (find_function_inject _ _ _ _ PRES H H8).
     intros (FINDFUN & KEPT). auto.
+    inv H. inv H1. simpl in H5. injg H5.
   - eapply match_states_call with (j := injw_meminj w); eauto.
     + inversion GE.
       constructor; eauto.
-      ++ inv H1; cbn in *. 
-         constructor; intros; try congruence. 
+      ++ inv H1; cbn in *.
+         constructor; intros; try congruence.
       ++ inv H1; cbn in *. auto.
       ++ inv H1; cbn in *. auto.
     + generalize (find_function_inject _ _ _ _ PRES H H8).
       intros (FINDFUN & KEPT). auto.
-=======
-  intros. inv H. exploit init_mem_inject; eauto. intros (tm & A & B & C).
-  exploit symbols_inject_2. eauto. eapply kept_main. eexact H1. intros (tb & P & Q).
-  rewrite Genv.find_funct_ptr_iff in H2.
-  exploit defs_inject. eauto. eexact Q. exact H2.
-  intros (R & S & T).
-  rewrite <- Genv.find_funct_ptr_iff in R.
-  exploit Genv.init_mem_stack; eauto. intro STK2.
-  exploit Genv.init_mem_stack. apply H0. intro STK1.
-  exploit Mem.alloc_parallel_inject; eauto. apply Z.le_refl. apply Z.le_refl.
-  intros (f' & tm' & b' & U &V &W&X&Y).
-  apply Mem.alloc_result in H4 as H5. unfold Mem.nextblock in H5. unfold fresh_block in H5.
-  rewrite STK1 in H5. simpl in H5. subst.
-  apply Mem.alloc_result in U as U'.  unfold Mem.nextblock in U'. unfold fresh_block in U'.
-  rewrite STK2 in U'. simpl in U'. subst.
-  apply Mem.valid_new_block in H4 as H6.
-  apply Mem.valid_new_block in U as U''.
-  apply Mem.stack_alloc in H4 as STK3. rewrite STK1 in STK3. simpl in STK3.
-  apply Mem.stack_alloc in U as STK4. rewrite STK2 in STK4. simpl in STK4.
-  exists (Callstate nil f nil tm' (prog_main tp)); split.
-  econstructor; eauto.
-  fold tge. erewrite match_prog_main by eauto. auto.
-  erewrite <- match_prog_main; eauto.
-  econstructor; eauto.
-  eapply match_stacks_bound. 2: eapply Mem.sup_include_alloc; eauto. 2: eapply Mem.sup_include_alloc; eauto.
-  eapply match_stacks_incr. eauto.
-  constructor. auto.
-  erewrite <- Genv.init_mem_genv_sup by eauto. apply Mem.sup_include_refl.
-  erewrite <- Genv.init_mem_genv_sup by eauto. apply Mem.sup_include_refl.
-  intros. destruct (eq_block b1 (Stack 1%positive)). subst. rewrite X in H5. inv H5.
-  simpl. rewrite STK1. rewrite STK2. simpl. split. lia. lia. rewrite Y in H5. congruence. auto.
-  erewrite Mem.astack_alloc. 2: eauto. apply Mem.astack_alloc in U. rewrite U.
-  erewrite Genv.init_mem_astack; eauto. erewrite Genv.init_mem_astack; eauto. constructor.
->>>>>>> origin/StackAware-new
+    + simpl. constructor. inv H1. inv ASTK. auto.
+    + inv H1. auto.
 Qed.
 
 Lemma transf_final_states:
@@ -1861,18 +1582,14 @@ Proof.
     + inv H0. constructor; auto.
     + constructor; auto.
       cbn. constructor; auto.
+      constructor. inv ASTK. auto.
 Qed.
 
-<<<<<<< HEAD
 Lemma transf_external_states:
   forall S R q1, match_states S R -> at_external ge S q1 ->
-  exists wx q2, at_external tge R q2 /\ match_query (cc_c inj) wx q1 q2 /\ match_senv (cc_c inj) wx se tse /\
-  forall r1 r2 S', match_reply (cc_c inj) wx r1 r2 -> after_external S r1 S' ->
+  exists wx q2, at_external tge R q2 /\ match_query (cc_c injp) wx q1 q2 /\ match_senv (cc_c injp) wx se tse /\
+  forall r1 r2 S', match_reply (cc_c injp) wx r1 r2 -> after_external S r1 S' ->
   exists R', after_external R r2 R' /\ match_states S' R'.
-=======
-Lemma transf_program_correct_1:
-  forward_simulation (semantics fn_stack_requirements p) (semantics fn_stack_requirements tp).
->>>>>>> origin/StackAware-new
 Proof.
   intros S R q1 MSTATE AT_EXT.
   inv AT_EXT. inv MSTATE.
@@ -1881,33 +1598,36 @@ Proof.
   intros PRES.
   generalize (find_function_inject _ _ _ _ PRES FUNINJ H).
   intros (FIND & KEPT1).
-  eexists (injw j (Mem.support m) (Mem.support tm)), _. intuition idtac.  
+  eexists (injpw j m tm MEMINJ), _. intuition idtac.
   - econstructor; eauto.
+    inv FUNINJ. injg H3.
   - econstructor; eauto. constructor. auto.
-    intros EQ. subst vf. inv FUNINJ. inv H.
+    constructor. eapply match_astack_size. eauto.
+    auto. congruence.
   - constructor.
     + eapply match_stacks_match_stbls; eauto.
     + eapply match_stacks_bound1; eauto.
     + eapply match_stacks_bound2; eauto.
-  - destruct H0 as (wx' & Hwx' & H'). inv Hwx'. inv H1. inv H'. eexists. split.
+  - destruct H1 as (wx' & Hwx' & H'). inv Hwx'. inv H2. inv H'. eexists. split.
     + econstructor; eauto.
-    + inv H6. econstructor; eauto. cbn.
-      apply match_stacks_incr_bound 
+      inv FUNINJ. injg H4.
+    + inv H5. econstructor; eauto. cbn.
+      apply match_stacks_incr_bound
         with (Mem.support m) (Mem.support tm); auto.
-      apply match_stacks_incr 
+      apply match_stacks_incr
         with j (Mem.support m) (Mem.support tm); auto.
+      inv UNCHANGED1. auto.
+      inv UNCHANGED2. auto.
+      congruence.
 Qed.
 
 End SOUNDNESS.
 
-<<<<<<< HEAD
-Theorem transf_program_correct prog tprog:
+End ORACLE.
+
+Theorem transf_program_correct prog tprog fn_stack_requirements:
   match_prog prog tprog ->
-  forward_simulation (cc_c inj) (cc_c inj) (semantics prog) (semantics tprog).
-=======
-Theorem transf_program_correct:
-  forall p tp, match_prog p tp -> forward_simulation (semantics fn_stack_requirements p) (semantics fn_stack_requirements tp).
->>>>>>> origin/StackAware-new
+  forward_simulation (cc_c injp) (cc_c inj) (semantics fn_stack_requirements prog) (semantics fn_stack_requirements tprog).
 Proof.
   intros MATCH.
   inv MATCH. destruct H as (VALID_USED & MATCH1).
@@ -1920,7 +1640,7 @@ Proof.
                Genv.find_symbol se1 (prog_main (skel prog)) = Some b ->
                exists b' : block, Genv.find_symbol se2 (prog_main (tskel tprog)) = Some b')
       as MAIN_SYM_PRES.
-    { 
+    {
       eapply main_symb_pres; eauto.
     }
     assert (forall (id : ident) (b : block),
@@ -1962,7 +1682,7 @@ Proof.
         inversion MSENV. exploit mge_dom; eauto. eapply Genv.genv_symb_range; eauto.
         intros [b3 INJ']. rewrite H5 in INJ'. inv INJ'.
         rewrite Ptrofs.add_zero.
-      
+
       unfold Genv.find_funct.
       unfold Genv.find_funct_ptr.
       destruct (Ptrofs.eq_dec i Ptrofs.zero); try congruence.
@@ -1994,16 +1714,16 @@ Proof.
       destruct ( Ptrofs.eq_dec i Ptrofs.zero); eauto.
     + intros q1 q2 s1 MQUERY INIT.
       eapply transf_initial_states with (se := se1) (tse := se2); eauto.
-      
+
     + intros s1 s2 r1 MSTATE FINAL.
       eapply transf_final_states with (se := se1) (tse := se2); eauto.
     + intros s1 s2 q1 MSTATE ATEXT.
       eapply transf_external_states; eauto.
     + intros s1 t s1' STEP s2 MSTATE.
       unfold semantics; cbn in *.
-      assert (exists s2', step (Genv.globalenv se2 tprog) s2 t s2' /\
+      assert (exists s2', step fn_stack_requirements (Genv.globalenv se2 tprog) s2 t s2' /\
                      match_states prog tprog used wB se1 se2 s1' s2') as GOAL.
-      { 
+      {
         apply step_simulation with (w:=wB) (S1:=s1); auto.
       }
       destruct GOAL as (s2' & STEP' & MSTATE').
@@ -2011,7 +1731,6 @@ Proof.
   - apply well_founded_ltof.
 Qed.
 
-End ORACLE.
 (** * Commutation with linking *)
 
 Remark link_def_either:
